\documentclass[a4paper,12pt,twoside]{article}
\usepackage[russian]{babel}
\usepackage[utf8]{inputenc}
 
\begin{document}

\begin{large} \textit{Задание 1.} Выполнить бета-редукцию $\lambda$-терма.\end{large} 
\newline

$((\lambda a.(\lambda b.b\;b)\;(\lambda b.b\;b))\;b)\;((\lambda c.(c\;b))\;(\lambda a.a)) \longrightarrow_{\beta} (\lambda b.b\;b)\;(\lambda b.b\;b)\;((\lambda c.(c\;b)\;(\lambda a.a))\longrightarrow_{\beta} (\lambda b.b\;b)\;(\lambda b.b\;b)\;((\lambda a.a)\;b) \longrightarrow_{\beta} (\lambda b.b\;b)\;(\lambda b.b\;b)\;b \longrightarrow_{\beta} (\lambda b.b\;b)\;(\lambda b.b\;b)\;b \longrightarrow_{\beta}~...$
\newline 

Данное $\lambda$-выражение не имеет нормальной формы.
\newline

\begin{large} \textit{Задание 2.} Доказать, что  S K K = I. \end{large} 
\newline

$S\;K\;K\;=\;(\lambda x\;y\;z.x\;z\;(y\;z))\;(\lambda x\;y.x)\;(\lambda x\;y.x) \longrightarrow_{\beta} \lambda z.(\lambda x\;y.x)\;z\;((\lambda x\;y.x)\;z) \longrightarrow_{\beta} \lambda z.(\lambda y.z)\;(\lambda y.z) \longrightarrow_{\beta} \lambda z.z\;=\;I$




\end{document}